FirstDescr.v
@@ -1,11 +1,11 @@
 Require Import Coq.Lists.List.
 Import ListNotations.
 
-Require Import Parser.Structures.
-Require Import Parser.List.
+Require Export Parser.Structures.
+Require Export Parser.List.
 
-Require Import Parser.NullableFun.
-Require Import Parser.ProductiveFun.
+Require Export Parser.NullableFun.
+Require Export Parser.ProductiveFun.
 
 Require Export Parser.Description.
 Require Export Parser.CommonRules.
@@ -13,7 +13,7 @@ Require Export Parser.CommonRules.
 Definition first_descr (k: token_class): Description (fun A => unit) := {|
   epsilon_descr := fun A a => [];
   failure_descr := fun A => [];
-  token_descr := fun k' => when_sum (class_eq_dec k k') [ some_rule tt ];
+  token_descr := fun k' => when_sum (kind_eq_dec k k') [ some_rule tt ];
   map_descr := fun _ _ _ _ _ => [ @id_rule unit ];
   disj_descr := fun _ _ _ => [ disj_rule ];
   seq_descr :=
