FocusedSyntaxLocateMatches.v
@@ -7,7 +7,7 @@ Lemma locate_sound_helper:
   forall n A (fs fs': Focused_Syntax A) t ts v,
     length (layers fs) + count_follow_by (layers fs) <= n ->
     matches (unfocus_helper (layers fs') (core fs')) (t :: ts) v ->
-    locate (class t) fs = Some fs' ->
+    locate (get_kind t) fs = Some fs' ->
     matches (unfocus_helper (layers fs) (core fs)) (t :: ts) v.
 Proof.
   induction n; destruct fs; intros; locate_def;
@@ -25,7 +25,7 @@ Qed.
 Lemma locate_sound:
   forall A (fs fs': Focused_Syntax A) t ts v,
     matches (unfocus_helper (layers fs') (core fs')) (t :: ts) v ->
-    locate (class t) fs = Some fs' ->
+    locate (get_kind t) fs = Some fs' ->
     matches (unfocus_helper (layers fs) (core fs)) (t :: ts) v.
 Proof.
   eauto using locate_sound_helper.
@@ -36,7 +36,7 @@ Lemma locate_complete_helper:
     length (layers fs) + count_follow_by (layers fs) <= n ->
     matches (unfocus_helper (layers fs) (core fs)) (t :: ts) v ->
     ~ has_conflict_ind (unfocus_helper (layers fs) (core fs)) ->
-    locate (class t) fs = Some fs' ->
+    locate (get_kind t) fs = Some fs' ->
     matches (unfocus_helper (layers fs') (core fs')) (t :: ts) v.
 Proof.
   induction n; destruct fs; intros; locate_def;
@@ -58,18 +58,28 @@ Lemma locate_complete:
   forall A (fs fs': Focused_Syntax A) t ts v,
     matches (unfocus_helper (layers fs) (core fs)) (t :: ts) v ->
     ~ has_conflict_ind (unfocus_helper (layers fs) (core fs)) ->
-    locate (class t) fs = Some fs' ->
+    locate (get_kind t) fs = Some fs' ->
     matches (unfocus_helper (layers fs') (core fs')) (t :: ts) v.
 Proof.
   eauto using locate_complete_helper.
 Qed.
 
+Lemma locate_correct:
+  forall A (fs fs': Focused_Syntax A) t,
+    locate (get_kind t) fs = Some fs' ->
+    ~ has_conflict_ind (unfocus_helper (layers fs) (core fs)) ->
+      forall ts v,
+      matches (unfocus_helper (layers fs') (core fs')) (t :: ts) v <->
+      matches (unfocus_helper (layers fs) (core fs)) (t :: ts) v.
+Proof.
+  lights; eauto using locate_sound, locate_complete.
+Qed.
+
 Lemma locate_not_none_helper:
   forall n A (fs: Focused_Syntax A) t ts v,
     length (layers fs) + count_follow_by (layers fs) <= n ->
-    locate (class t) fs = None ->
+    locate (get_kind t) fs = None ->
     matches (unfocus fs) (t :: ts) v ->
-    ~ has_conflict_ind (unfocus fs) ->
     False.
 Proof.
   unfold unfocus;
@@ -83,18 +93,18 @@ Proof.
     try solve [ eapply_anywhere plug_no_conflict_unfocus; eauto ];
     try solve [ rewrite_any; lights ].
 
+  - apply (matches_unfocus_helper_sub_first3 _ _ _ _ (Epsilon i)) in H1;
+      lights;
+      eauto with matches;
+      eauto using first_fun_complete with exfalso.
 
-  - eapply IHn in H0;
+    eapply IHn in H0;
       eauto;
       try solve [ intros; eapply_anywhere plug_no_conflict_unfocus; eauto ].
     + unshelve epose proof (plug_count_follow_by _ _ layers i _); lights.
       unfold plug in *; lia.
 
     + apply plug_complete; unfold unfocus; lights; eauto.
-      eapply matches_unfocus_propagate_first;
-        eauto; repeat light || invert_matches || nullable_fun_spec;
-          eauto with matches;
-          eauto with exfalso unfocus_conflict_more.
 
   - matches_unfocus_helper_prefix;
       repeat light || app_cons_destruct || invert_constructor_equalities;
@@ -103,22 +113,30 @@ Qed.
 
 Lemma locate_not_none:
   forall A (fs: Focused_Syntax A) t ts v,
-    locate (class t) fs = None ->
+    locate (get_kind t) fs = None ->
     matches (unfocus fs) (t :: ts) v ->
-    ~ has_conflict_ind (unfocus fs) ->
     False.
 Proof.
   eauto using locate_not_none_helper.
 Qed.
 
+Lemma locate_not_none2:
+  forall A (fs: Focused_Syntax A) k,
+    locate k fs = None ->
+    ~ first_ind (unfocus fs) k.
+Proof.
+  lights.
+  apply_anywhere first_ind_sound; lights.
+  eauto using locate_not_none.
+Qed.
+
 Lemma locate_is_some:
   forall A (fs: Focused_Syntax A) t ts v,
     matches (unfocus fs) (t :: ts) v ->
-    ~ has_conflict_ind (unfocus fs) ->
-    is_some (locate (class t) fs).
+    is_some (locate (get_kind t) fs).
 Proof.
   intros.
-  destruct (locate (class t) fs) eqn:L;
+  destruct (locate (get_kind t) fs) eqn:L;
     repeat light || options;
     eauto using locate_not_none.
 Qed.
