HasConflictDescr.v
@@ -1,10 +1,10 @@
 Require Import Coq.Lists.List.
 Import ListNotations.
 
-Require Import Parser.Option.
-Require Import Parser.List.
-Require Import Parser.DescriptionToFunctionSoundness.
-Require Import Parser.DescriptionToFunctionCompleteness.
+Require Export Parser.Option.
+Require Export Parser.List.
+Require Export Parser.DescriptionToFunctionSoundness.
+Require Export Parser.DescriptionToFunctionCompleteness.
 
 Require Export  Parser.NullableFun.
 Require Export Parser.ProductiveFun.
@@ -19,10 +19,10 @@ Definition has_conflict_descr: Description (fun A => unit) := {|
   map_descr := fun _ _ _ _ _ => [ @id_rule unit ];
   disj_descr := fun _ s1 s2 =>
     left_rule :: right_rule ::
-    when (negb (disjoint class_eq_dec (first_fun s1) (first_fun s2))) [ some_rule tt ] ++
+    when (negb (disjoint kind_eq_dec (first_fun s1) (first_fun s2))) [ some_rule tt ] ++
     when (is_some_b (nullable_fun s1) && is_some_b (nullable_fun s2)) [ some_rule tt ];
   seq_descr := fun _ _ s1 s2 =>
     left_rule :: right_rule ::
-    when (negb (disjoint class_eq_dec (should_not_follow_fun s1) (first_fun s2))) [ some_rule tt ];
+    when (negb (disjoint kind_eq_dec (should_not_follow_fun s1) (first_fun s2))) [ some_rule tt ];
   var_descr := fun _ _ => [ @id_rule unit ];
 |}.
