MatchesInversions.v
@@ -6,7 +6,7 @@ Require Export Parser.AmbiguityConflict.
 Lemma matches_inv_disj_l:
   forall A (s1 s2 : Syntax A) t ts v,
     matches (Disjunction s1 s2) (t :: ts) v ->
-    In (class t) (first_fun s1) ->
+    In (get_kind t) (first_fun s1) ->
     (has_conflict_ind (Disjunction s1 s2) -> False) ->
     matches s1 (t :: ts) v.
 Proof.
@@ -17,7 +17,7 @@ Qed.
 Lemma matches_inv_disj_r:
   forall A (s1 s2 : Syntax A) t ts v,
     matches (Disjunction s1 s2) (t :: ts) v ->
-    In (class t) (first_fun s2) ->
+    In (get_kind t) (first_fun s2) ->
     (has_conflict_ind (Disjunction s1 s2) -> False) ->
     matches s2 (t :: ts) v.
 Proof.
@@ -28,7 +28,7 @@ Qed.
 Lemma matches_inv_seq:
   forall A1 A2 (s1: Syntax A1) (s2 : Syntax A2) t ts v a,
     matches (Sequence s1 s2) (t :: ts) v ->
-    ~In (class t) (first_fun s1) ->
+    ~In (get_kind t) (first_fun s1) ->
     matches s1 [] a ->
     (has_conflict_ind (Sequence s1 s2) -> False) ->
     matches (Sequence (Epsilon a) s2) (t :: ts) v.
