ProductiveInd.v
@@ -1,7 +1,7 @@
-Require Import Parser.DescriptionInd.
-Require Import Parser.Structures.
-Require Import Parser.Matches.
-Require Import Parser.ProductiveDescr.
+Require Export Parser.DescriptionInd.
+Require Export Parser.Structures.
+Require Export Parser.Matches.
+Require Export Parser.ProductiveDescr.
 
 Definition productive_ind { A } (s: Syntax A): Prop := descr_ind productive_descr s tt.
 
@@ -28,7 +28,5 @@ Lemma productive_ind_correct:
   forall A (s: Syntax A),
     productive_ind s <-> (exists xs v, matches s xs v).
 Proof.
-  lights;
-    eauto using productive_ind_sound;
-    eauto using productive_ind_complete.
+  lights; eauto using productive_ind_sound, productive_ind_complete.
 Qed.
