ShouldNotFollowDescr.v
@@ -1,9 +1,9 @@
 Require Import Coq.Lists.List.
 Import ListNotations.
 
-Require Import Parser.Structures.
-Require Import Parser.Option.
-Require Import Parser.List.
+Require Export Parser.Structures.
+Require Export Parser.Option.
+Require Export Parser.List.
 Require Export Parser.DescriptionInd.
 Require Export Parser.CommonRules.
 Require Export Parser.NullableFun.
@@ -21,8 +21,8 @@ Definition should_not_follow_descr (k: token_class): Description (fun A => unit)
   map_descr := fun _ _ _ _ _ => [ @id_rule unit ];
   disj_descr := fun _ s1 s2 =>
     [ disj_rule ] ++
-    when_opt (nullable_fun s2) (when_sum (in_dec class_eq_dec k (first_fun s1)) [ some_rule tt ])  ++
-    when_opt (nullable_fun s1) (when_sum (in_dec class_eq_dec k (first_fun s2)) [ some_rule tt ]);
+    when_opt (nullable_fun s2) (when_sum (in_dec kind_eq_dec k (first_fun s1)) [ some_rule tt ])  ++
+    when_opt (nullable_fun s1) (when_sum (in_dec kind_eq_dec k (first_fun s2)) [ some_rule tt ]);
   seq_descr :=
     fun _ _ s1 s2 =>
       when_opt (nullable_fun s2) [ left_rule ] ++
